\documentclass{beamer}
\usetheme{Madrid}

\providecommand{\pr}[1]{\ensuremath{\Pr\left(#1\right)}}
\providecommand{\prt}[2]{\ensuremath{p_{#1}^{\left(#2\right)} }}        % own macro for this question
\providecommand{\qfunc}[1]{\ensuremath{Q\left(#1\right)}}
\providecommand{\sbrak}[1]{\ensuremath{{}\left[#1\right]}}
\providecommand{\lsbrak}[1]{\ensuremath{{}\left[#1\right.}}
\providecommand{\rsbrak}[1]{\ensuremath{{}\left.#1\right]}}
\providecommand{\brak}[1]{\ensuremath{\left(#1\right)}}
\providecommand{\lbrak}[1]{\ensuremath{\left(#1\right.}}
\providecommand{\rbrak}[1]{\ensuremath{\left.#1\right)}}
\providecommand{\cbrak}[1]{\ensuremath{\left\{#1\right\}}}
\providecommand{\lcbrak}[1]{\ensuremath{\left\{#1\right.}}
\providecommand{\rcbrak}[1]{\ensuremath{\left.#1\right\}}}
\newcommand{\sgn}{\mathop{\mathrm{sgn}}}
\providecommand{\abs}[1]{\left\vert#1\right\vert}
\providecommand{\res}[1]{\Res\displaylimits_{#1}} 
\providecommand{\norm}[1]{\left\lVert#1\right\rVert}
%\providecommand{\norm}[1]{\lVert#1\rVert}
\providecommand{\mtx}[1]{\mathbf{#1}}
\providecommand{\mean}[1]{E\left[ #1 \right]}
\providecommand{\cond}[2]{#1\middle|#2}
\providecommand{\fourier}{\overset{\mathcal{F}}{ \rightleftharpoons}}
%\providecommand{\hilbert}{\overset{\mathcal{H}}{ \rightleftharpoons}}
%\providecommand{\system}{\overset{\mathcal{H}}{ \longleftrightarrow}}
	%\newcommand{\solution}[2]{\textbf{Solution:}{#1}}
%\newcommand{\solution}{\noindent \textbf{Solution: }}
\newcommand{\cosec}{\,\text{cosec}\,}
\providecommand{\dec}[2]{\ensuremath{\overset{#1}{\underset{#2}{\gtrless}}}}
\newcommand{\myvec}[1]{\ensuremath{\begin{pmatrix}#1\end{pmatrix}}}
\newcommand{\mydet}[1]{\ensuremath{\begin{vmatrix}#1\end{vmatrix}}}
\providecommand{\rank}{\text{rank}}
\providecommand{\pr}[1]{\ensuremath{\Pr\left(#1\right)}}
\providecommand{\qfunc}[1]{\ensuremath{Q\left(#1\right)}}
	\newcommand*{\permcomb}[4][0mu]{{{}^{#3}\mkern#1#2_{#4}}}
\newcommand*{\perm}[1][-3mu]{\permcomb[#1]{P}}
\newcommand*{\comb}[1][-1mu]{\permcomb[#1]{C}}
\providecommand{\qfunc}[1]{\ensuremath{Q\left(#1\right)}}
\providecommand{\gauss}[2]{\mathcal{N}\ensuremath{\left(#1,#2\right)}}
\providecommand{\diff}[2]{\ensuremath{\frac{d{#1}}{d{#2}}}}
\providecommand{\myceil}[1]{\left \lceil #1 \right \rceil }
\newcommand\figref{Fig.~\ref}
\newcommand\tabref{Table~\ref}
\newcommand{\sinc}{\,\text{sinc}\,}
\newcommand{\rect}{\,\text{rect}\,}
\newcommand{\BEQA}{\begin{eqnarray}}
\newcommand{\EEQA}{\end{eqnarray}}
\newcommand{\define}{\stackrel{\triangle}{=}}
\bibliographystyle{IEEEtran}
\providecommand{\mbf}{\mathbf}
\providecommand{\pr}[1]{\ensuremath{\Pr\left(#1\right)}}
\providecommand{\qfunc}[1]{\ensuremath{Q\left(#1\right)}}
\providecommand{\sbrak}[1]{\ensuremath{{}\left[#1\right]}}
\providecommand{\lsbrak}[1]{\ensuremath{{}\left[#1\right.}}
\providecommand{\rsbrak}[1]{\ensuremath{{}\left.#1\right]}}
\providecommand{\brak}[1]{\ensuremath{\left(#1\right)}}
\providecommand{\lbrak}[1]{\ensuremath{\left(#1\right.}}
\providecommand{\rbrak}[1]{\ensuremath{\left.#1\right)}}
\providecommand{\cbrak}[1]{\ensuremath{\left\{#1\right\}}}
\providecommand{\lcbrak}[1]{\ensuremath{\left\{#1\right.}}
\providecommand{\rcbrak}[1]{\ensuremath{\left.#1\right\}}}
\theoremstyle{remark}
\newtheorem{rem}{Remark}
\providecommand{\abs}[1]{\left\vert#1\right\vert}
\providecommand{\res}[1]{\Res\displaylimits_{#1}} 
\providecommand{\norm}[1]{\left\lVert#1\right\rVert}
\providecommand{\mtx}[1]{\mathbf{#1}}
\providecommand{\mean}[1]{E\left[ #1 \right]}
\providecommand{\fourier}{\overset{\mathcal{F}}{ \rightleftharpoons}}
\providecommand{\system}[1]{\overset{\mathcal{#1}}{ \longleftrightarrow}}
\providecommand{\dec}[2]{\ensuremath{\overset{#1}{\underset{#2}{\gtrless}}}}
\let\vec\mathbf
\def\putbox#1#2#3{\makebox[0in][l]{\makebox[#1][l]{}\raisebox{\baselineskip}[0in][0in]{\raisebox{#2}[0in][0in]{#3}}}}
     \def\rightbox#1{\makebox[0in][r]{#1}}
     \def\centbox#1{\makebox[0in]{#1}}
     \def\topbox#1{\raisebox{-\baselineskip}[0in][0in]{#1}}
     \def\midbox#1{\raisebox{-0.5\baselineskip}[0in][0in]{#1}}
\title 
{GATE 2023 ST 17}
\author{Barath Surya}
\institute{IITH}
\date{2023}

\begin{document}

\frame{\titlepage}

\begin{frame}
\frametitle{Question}
Let $X$ be a random variable having Poisson distribution with mean $\lambda>0$. Then E\brak{\cond{\frac{1}{1+X}}{X>0}} equals
\begin{enumerate}
	\item $\frac{1-e^{-\lambda}-\lambda e^{-\lambda}}{\lambda\brak{1-e^{-\lambda}}}$
	\item $\frac{1-e^{-\lambda}}{\lambda}$
	\item $\frac{1-e^{-\lambda}-\lambda e^{-\lambda}}{\lambda}$
	\item $\frac{1-e^{-\lambda}}{\lambda +1}$
\end{enumerate}
\end{frame}
\begin{frame}
    \frametitle{Defining Poisson random variable}
    Let $X$ be a Poisson random variable, then pmf of $X$ is defined as
    \begin{align}
        X&\sim Pois\brak{\lambda}\\
        \pr{X=k}&=e^{-\lambda} \frac{\lambda^k}{k!}; k \geq 0 \label{eq:poissondistributionpmf}
    \end{align}
    where $\lambda$ is the Poisson parameter and also,
    \begin{align}
        E\brak{X}&=\lambda
    \end{align}
\end{frame}
\begin{frame}
    \frametitle{Conditional Expectance}
    Conditional Expectance $E\brak{X|Y}$ is defined as
    \begin{align}
        E\brak{X\mid A}&=\sum _{x}xP\brak{X=x\mid A}\\
        &=\sum _{x}x{\frac {P\brak{X=x, A}}{P\brak{A}}}\\
        \implies E\brak{\cond{\frac{1}{1+X}}{X>0}} &=\frac{\sum_{k=1}^{\infty}\frac{1}{k+1}\pr{X=k}}{\pr{X>0}}\\
        &=\frac{\sum_{k=1}^{\infty}\frac{1}{k+1} e^{-\lambda}\frac{\lambda^k}{k!}}{1-\pr{X\leq 0}}\\
        &=\frac{e^{-\lambda}\sum_{k=1}^{\infty}\frac{\lambda^k}{\brak{k+1}!}}{1-\pr{X=0}}
    \end{align}
\end{frame}
\begin{frame}
    from equation \eqref{eq:poissondistributionpmf}
\begin{align}
	&=\frac{e^{-\lambda}\sum_{k=1}^{\infty}\frac{\lambda^k}{\brak{k+1}!}}{1-e^{\lambda}}
\end{align}
Now simplifying Just the Summation
\begin{align}
	\implies & \sum_{k=1}^{\infty} \frac{\lambda^k}{\brak{k+1}!}\\
	&=\frac{1}{\lambda} \sum_{k=1}^{\infty} \frac{\lambda^{k+1}}{k+1}
\end{align}
Letting $k+1 =m $,
\begin{align}
	\implies & \frac{1}{\lambda} \sum_{m=2}^{\infty} \frac{\lambda^m}{m!}
\end{align}
\end{frame}
\begin{frame}
    We Know from Taylor series
\begin{align}
	e^x&=\sum_{k=0}^{\infty} \frac{x^k}{k!}\\
	\implies \frac{1}{\lambda} \sum_{m=2}^{\infty} \frac{\lambda^m}{m!}&= \frac{1}{\lambda}\brak{e^{\lambda}-1-\lambda}
\end{align}
Substituting back we get,
\begin{align}
	&=\frac{e^{-\lambda}}{ \brak{1-e^{\lambda}}}\brak{\frac{1}{\lambda} \brak{e^{\lambda}-1-\lambda}}\\
	&=\frac{e^{-\lambda}}{\lambda \brak{1-e^{\lambda}}}\brak{e^{\lambda}-1 -\lambda}\\
	&=\frac{1-e^{-\lambda}-\lambda e^{-\lambda}}{\lambda \brak{1-e^{\lambda}}}
\end{align}
\end{frame}
\end{document}